experiment/Experiment.Steel.Repr.LV_to_SF.fsti
@@ -30,6 +30,10 @@ let rec repr_SF_of_LV
                   repr_SF_of_LV (cg x) (res_sel sl0 f_csm sl1))
   | LCbindP env #a #b #wp #g csm prd cg ->
       SF.TbindP a b (M.post_sl_t prd) wp (fun (x : a) -> repr_SF_of_LV (cg x) sl0)
+  | LCif    env #a #guard #thn #els csm prd cthn cels ->
+      SF.Tif   a guard (M.post_sl_t prd)
+               (repr_SF_of_LV cthn sl0)
+               (repr_SF_of_LV cels sl0)
   | LCsub  env csm0 prd0 cf csm1 prd1 prd_f ->
       SF.Tbind a a (M.post_sl_t prd0) (M.post_sl_t prd1)
                (repr_SF_of_LV cf sl0)
